WIP

Bdd/Sim.lean
@@ -2,8 +2,300 @@ module
 
 public import Bdd.Basic
 import Std.Data.HashMap.Lemmas
+import Std.Tactic.Do
+open Std.Do
 
 namespace Sim
+
+structure State m m' where
+  lr : Std.HashMap (Fin m) (Fin m')
+  rl : Std.HashMap (Fin m') (Fin m)
+
+def sim_helper' {n m m'}
+    (O : OBdd n m) (hO : OBdd.Reduced O)
+    (U : OBdd n m') (hU : OBdd.Reduced U)
+    (p : Pointer m) (hpr : Pointer.Reachable O.1.heap O.1.root p)
+    (q : Pointer m') (hqr : Pointer.Reachable U.1.heap U.1.root q) :
+    State m m' → (State m m') × Bool :=
+  fun s => match p, q with
+  | .terminal b, .terminal b' => (s, b = b')
+  | .terminal _, .node _ => (s, false)
+  | .node _, .terminal _ => (s, false)
+  | .node j, .node j' =>
+    if hv : O.1.heap[j].var = U.1.heap[j'].var
+    then
+      match s.lr[j]? with
+      | some i' => (s, j' = i')
+      | none =>
+        match s.rl[j']? with
+        | some i => (s, false)
+        | none =>
+          let (sl, bl) := sim_helper' O hO U hU
+            O.1.heap[j].low (.snoc hpr .low) U.1.heap[j'].low (.snoc hqr .low) s
+          if bl then
+            let (sh, bh) := sim_helper' O hO U hU
+              O.1.heap[j].high (.snoc hpr .high) U.1.heap[j'].high (.snoc hqr .high) sl
+            if bh then
+              (⟨s.lr.insert j j', s.rl.insert j' j⟩, true)
+            else
+              (sh, false)
+          else (sl, false)
+    else (s, false)
+termination_by OBdd.size' ⟨⟨O.1.heap, p⟩, O.ordered_of_reachable hpr⟩
+decreasing_by
+  · simp [OBdd.size'_node, OBdd.low_eq, Bdd.low_eq]; omega
+  · simp [OBdd.size'_node, OBdd.high_eq, Bdd.high_eq]; omega
+
+def sim_helper {n m m'}
+    (O : OBdd n m) (hO : OBdd.Reduced O)
+    (U : OBdd n m') (hU : OBdd.Reduced U)
+    (p : Pointer m) (hpr : Pointer.Reachable O.1.heap O.1.root p)
+    (q : Pointer m') (hqr : Pointer.Reachable U.1.heap U.1.root q) :
+    StateM (State m m') Bool :=
+  match p, q with
+  | .terminal b, .terminal b' => return b = b'
+  | .terminal _, .node _ => return false
+  | .node _, .terminal _ => return false
+  | .node j, .node j' =>
+    if hv : O.1.heap[j].var = U.1.heap[j'].var
+    then do
+      let s ← get
+      match s.lr[j]? with
+      | some i' => return j' = i'
+      | none =>
+        match s.rl[j']? with
+        | some i => return false
+        | none =>
+          let hll ← sim_helper O hO U hU
+            O.1.heap[j].low (.snoc hpr .low) U.1.heap[j'].low (.snoc hqr .low)
+          if hll then
+            let hhh ← sim_helper O hO U hU
+              O.1.heap[j].high (.snoc hpr .high) U.1.heap[j'].high (.snoc hqr .high)
+            match hhh with
+            | true =>
+              set <| State.mk (s.lr.insert j j') (s.rl.insert j' j)
+              return true
+            | false => return false
+          else return false
+    else return false
+termination_by OBdd.size' ⟨⟨O.1.heap, p⟩, O.ordered_of_reachable hpr⟩
+decreasing_by
+  · simp [OBdd.size'_node, OBdd.low_eq, Bdd.low_eq]; omega
+  · simp [OBdd.size'_node, OBdd.high_eq, Bdd.high_eq]; omega
+
+structure Invariant {n m m'} (O : OBdd n m) (U : OBdd n m') (s : State m m') where
+  hl : ∀ j j',
+    s.lr[j]? = some j' → s.rl[j']? = some j           ∧
+    Pointer.Reachable O.1.heap O.1.root (.node j) ∧
+    ∃ hj : Bdd.Ordered ⟨O.1.heap, .node j⟩,
+      ∃ hj' : Bdd.Ordered ⟨U.1.heap, .node j'⟩,
+        OBdd.HSimilar ⟨⟨O.1.heap, .node j⟩, hj⟩ ⟨⟨U.1.heap, .node j'⟩, hj'⟩
+  hr : ∀ j j',
+    s.rl[j']? = some j → s.lr[j]? = some j'            ∧
+    Pointer.Reachable U.1.heap U.1.root (.node j') ∧
+    ∃ hj : Bdd.Ordered ⟨O.1.heap, .node j⟩,
+      ∃ hj' : Bdd.Ordered ⟨U.1.heap, .node j'⟩,
+        OBdd.HSimilar ⟨⟨O.1.heap, .node j⟩, hj⟩ ⟨⟨U.1.heap, .node j'⟩, hj'⟩
+
+lemma sim_helper_invariant {n m m'}
+    (O : OBdd n m) (hO : OBdd.Reduced O)
+    (U : OBdd n m') (hU : OBdd.Reduced U)
+    (p : Pointer m) (hpr : Pointer.Reachable O.1.heap O.1.root p)
+    (q : Pointer m') (hqr : Pointer.Reachable U.1.heap U.1.root q) {b s s'} :
+    (sim_helper O hO U hU p hpr q hqr).run s = pure (b, s') →
+    Invariant O U s → Invariant O U s' := by
+  fun_induction sim_helper generalizing s s' with
+  | case4 j j' hr1 hr2 heq1 hr3 hr4 ih1 ih2 =>
+    simp only [bind_pure_comp, StateT.run_bind, StateT.run_get, pure_bind]
+    split
+    · rintro ⟨rfl, rfl⟩; simp only [imp_self]
+    split
+    · rintro ⟨rfl, rfl⟩; simp only [imp_self]
+    simp_all only [StateT.run, getElem?_eq_none_iff, bind, StateT.bind]
+    split
+    split
+    · simp_all only [bind, StateT.bind]
+      split
+      split
+      ·
+        sorry
+      · rintro ⟨rfl, rfl⟩
+        have := ih1 (by assumption)
+        have := ih2 (by assumption)
+        sorry
+    · rintro ⟨rfl, rfl⟩
+      sorry
+  | _ =>
+    rintro ⟨rfl, rfl⟩
+    simp only [imp_self]
+
+
+lemma sim_helper_invariant' {n m m'}
+    (O : OBdd n m) (hO : OBdd.Reduced O)
+    (U : OBdd n m') (hU : OBdd.Reduced U)
+    (p : Pointer m) (hpr : Pointer.Reachable O.1.heap O.1.root p)
+    (q : Pointer m') (hqr : Pointer.Reachable U.1.heap U.1.root q) {b s s'} :
+    (sim_helper O hO U hU p hpr q hqr).run s = pure (b, s') →
+    Invariant O U s → Invariant O U s' := by
+  generalize h : (sim_helper O hO U hU p hpr q hqr).run s = x
+  apply StateM.of_wp_run_eq h
+  mvcgen
+  intro heq i
+
+  sorry
+
+lemma sim_helper_correct {n m m'}
+    (O : OBdd n m) (hO : OBdd.Reduced O)
+    (U : OBdd n m') (hU : OBdd.Reduced U)
+    (p : Pointer m) (hpr : Pointer.Reachable O.1.heap O.1.root p)
+    (q : Pointer m') (hqr : Pointer.Reachable U.1.heap U.1.root q) {b s} :
+    (sim_helper O hO U hU p hpr q hqr).run ⟨∅, ∅⟩ = pure (b, s) ↔ O.HSimilar U := by
+  generalize h : (sim_helper O hO U hU p hpr q hqr).run ⟨∅, ∅⟩ = x
+  apply StateM.of_wp_run_eq h
+  mvcgen
+  sorry
+/-  match hp : p with
+  | .terminal b =>
+    match hq : q with
+    | .terminal b' =>
+      if hb : b = b'
+      then return isTrue (by simpa [OBdd.HSimilar, OBdd.toTree_terminal])
+      else return isFalse (by simpa [OBdd.HSimilar, OBdd.toTree_terminal])
+    | .node j' => return isFalse (by simp [OBdd.HSimilar, OBdd.toTree_terminal, OBdd.toTree_node])
+  | .node j =>
+    match hq : q with
+    | .terminal b' => return isFalse (by simp [OBdd.HSimilar, OBdd.toTree_terminal, OBdd.toTree_node])
+    | .node j' =>
+      if hv : O.1.heap[j].var = U.1.heap[j'].var
+      then do
+        let s ← get
+        match hl : s.lr[j]? with
+        | none =>
+          match hr : s.rl[j']? with
+          | none =>
+            let hll ← sim_helper O hO U hU
+              O.1.heap[j].low (Pointer.Reachable.snoc hpr .low)
+              U.1.heap[j'].low (Pointer.Reachable.snoc hqr .low)
+            match hll with
+            | isTrue ht =>
+              -- TODO : why is type declaration needed? Note that only `←` does not work, for some reason `:= ←` is needed
+              let hhh : Decidable (OBdd.HSimilar ⟨Bdd.mk O.bdd.heap O.bdd.heap[j].high, _⟩ ⟨Bdd.mk U.bdd.heap U.bdd.heap[j'].high, _⟩) :=
+                ← sim_helper O hO U hU
+                O.1.heap[j].high (Pointer.Reachable.snoc hpr .high)
+                U.1.heap[j'].high (Pointer.Reachable.snoc hqr .high)
+              match hhh with
+              | isTrue ht' =>
+                set
+                  (⟨s.lr.insert j j', s.rl.insert j' j,
+                    fun jj jj' hjj ↦ by
+                      simp only [Std.HashMap.getElem?_insert, beq_iff_eq] at hjj
+                      split at hjj
+                      next heq =>
+                        subst heq
+                        simp only [Std.HashMap.getElem?_insert, beq_iff_eq]
+                        split
+                        next heqq =>
+                          subst heqq
+                          simp only [true_and]
+                          constructor
+                          · exact hpr
+                          · use OBdd.ordered_of_reachable hpr
+                            use OBdd.ordered_of_reachable hqr
+                            simp only [OBdd.HSimilar] at ⊢ ht ht'
+                            rw [OBdd.toTree_node rfl, OBdd.toTree_node (j := j') rfl]
+                            simp only [OBdd.low_eq, Bdd.low_eq, OBdd.high_eq, Bdd.high_eq,
+                              DecisionTree.branch.injEq]
+                            exact ⟨hv, ht, ht'⟩
+                        next heqq => injection hjj; contradiction
+                      next heq =>
+                        simp only [Std.HashMap.getElem?_insert, beq_iff_eq]
+                        split
+                        next heqq =>
+                          subst heqq
+                          rw [(s.hl jj j' hjj).1] at hr
+                          contradiction
+                        next heqq =>
+                          exact s.hl jj jj' hjj,
+                    fun jj jj' hjj ↦ by
+                      simp only [Std.HashMap.getElem?_insert, beq_iff_eq] at hjj
+                      split at hjj
+                      next heq =>
+                        subst heq
+                        simp only [Std.HashMap.getElem?_insert, beq_iff_eq]
+                        split
+                        next heqq =>
+                          subst heqq
+                          simp only [true_and]
+                          constructor
+                          · exact hqr
+                          · use OBdd.ordered_of_reachable hpr
+                            use OBdd.ordered_of_reachable hqr
+                            simp only [OBdd.HSimilar] at ⊢ ht ht'
+                            rw [OBdd.toTree_node rfl, OBdd.toTree_node (j := j') rfl]
+                            simp only [OBdd.low_eq, Bdd.low_eq, OBdd.high_eq, Bdd.high_eq,
+                              DecisionTree.branch.injEq]
+                            exact ⟨hv, ht, ht'⟩
+                        next heqq => injection hjj; contradiction
+                      next heq =>
+                        simp only [Std.HashMap.getElem?_insert, beq_iff_eq]
+                        split
+                        next heqq =>
+                          subst heqq
+                          rw [(s.hr j jj' hjj).1] at hl
+                          contradiction
+                        next heqq =>
+                          exact s.hr jj jj' hjj
+                   ⟩ : State O U)
+                return isTrue (by
+                  simp only [OBdd.HSimilar] at ⊢ ht ht'
+                  rw [OBdd.toTree_node rfl, OBdd.toTree_node (j := j') rfl]
+                  simp only [OBdd.low_eq, Bdd.low_eq, OBdd.high_eq, Bdd.high_eq,
+                    DecisionTree.branch.injEq]
+                  exact ⟨hv, ht, ht'⟩
+                )
+              | isFalse hf' => return isFalse (fun c ↦ by
+                simp [OBdd.HSimilar, OBdd.toTree_node, OBdd.high_eq, Bdd.high_eq] at c;
+                exact hf' c.2.2)
+            | isFalse hf => return isFalse (fun c ↦ by
+              simp [OBdd.HSimilar, OBdd.toTree_node, OBdd.low_eq, Bdd.low_eq] at c; exact hf c.2.1)
+          | some i =>
+            return isFalse (by
+              rcases s.hr i j' hr with ⟨h1, h2, h3, h4, h5⟩
+              rcases s.hl i j' h1 with ⟨h1', h2', h3', h4', h5'⟩
+              intro contra
+              have hsim : OBdd.SimilarRP O ⟨.node i, h2'⟩ ⟨.node j, hpr⟩ := by
+                simp [OBdd.similarRP_iff]
+                simp only [OBdd.HSimilar] at contra h5
+                rw [contra]
+                exact h5
+              have h := hO.2 hsim
+              simp [InvImage] at h
+              subst h
+              rw [h1] at hl
+              contradiction
+            )
+        | some i' =>
+          if heq : j' = i'
+          then
+            return isTrue (s.hl j j' (by simp_all)).2.2.2.2
+          else
+            return isFalse (fun c ↦ heq (by
+              rcases s.hl j i' hl with ⟨h1, h2, h3, h4, h5⟩
+              rcases s.hr j i' h1 with ⟨h1', h2', h3', h4', h5'⟩
+              have hsim : OBdd.SimilarRP U ⟨.node j', hqr⟩ ⟨.node i', h2'⟩ := by
+                simp [OBdd.similarRP_iff]
+                simp only [OBdd.HSimilar] at c h5
+                rw [c] at h5
+                exact h5
+              have := hU.2 hsim
+              simp [InvImage] at this
+              exact this
+            ))
+      else return isFalse (by simp_all [OBdd.HSimilar, OBdd.toTree_node])
+termination_by OBdd.size' ⟨⟨O.1.heap, p⟩, O.ordered_of_reachable hpr⟩
+decreasing_by
+  · simp [OBdd.size'_node, OBdd.low_eq, Bdd.low_eq]; omega
+  · simp [OBdd.size'_node, OBdd.high_eq, Bdd.high_eq]; omega-/
 
 structure State {n m m'} (O : OBdd n m) (U : OBdd n m') where
   lr : Std.HashMap (Fin m) (Fin m')
@@ -21,7 +313,7 @@ structure State {n m m'} (O : OBdd n m) (U : OBdd n m') where
       ∃ hj' : Bdd.Ordered ⟨U.1.heap, .node j'⟩,
         OBdd.HSimilar ⟨⟨O.1.heap, .node j⟩, hj⟩ ⟨⟨U.1.heap, .node j'⟩, hj'⟩
 
-def sim_helper {n m m'}
+def sim_helper' {n m m'}
     (O : OBdd n m) (hO : OBdd.Reduced O)
     (U : OBdd n m') (hU : OBdd.Reduced U)
     (p : Pointer m) (hpr : Pointer.Reachable O.1.heap O.1.root p)
